theories/logrel/examples/compute_service.v
@@ -1,0 +1,74 @@
+From iris.algebra Require Import frac.
+From iris.heap_lang Require Import metatheory.
+From actris.utils Require Import llist.
+From actris.channel Require Import proofmode proto channel.
+From actris.logrel Require Import term_typing_rules session_typing_rules
+     subtyping_rules napp.
+From actris.logrel.lib Require Import par_start.
+
+Definition cont : Z := 1.
+Definition stop : Z := 2.
+
+Definition compute_service : val :=
+  rec: "go" "c":=
+    branch [cont;stop] "c"
+    (λ: "c", let: "v" := recv "c" in
+             send "c" ("v" #());; "go" "c")
+    (λ: "c", #()).
+ 
+Section compute_example.
+  Context `{heapG Σ, chanG Σ, spawnG Σ}.
+
+  Definition compute_type_service_aux (rec : lsty Σ) : lsty Σ :=
+    lty_branch $ <[cont := (<?? A> TY () ⊸ A; <!!> TY A ; rec)%lty]> $
+                 <[stop := END%lty]> $ ∅.
+  Instance mapper_type_rec_service_contractive :
+    Contractive (compute_type_service_aux).
+  Proof. solve_proto_contractive. Qed.
+  Definition compute_type_service : lsty Σ :=
+    lty_rec (compute_type_service_aux).
+
+  (** This judgement is checked only with the typing rules of the type system *)
+  Lemma ltyped_compute_service Γ :
+    ⊢ Γ ⊨ compute_service : lty_chan compute_type_service ⊸ () ⫤ Γ.
+  Proof.
+    iApply (ltyped_subsumption _ _ _ _ _ _
+              (lty_chan compute_type_service → ())%lty);
+      [ iApply env_le_refl | iApply lty_le_copy_elim | iApply env_le_refl | ].
+    iApply ltyped_val_ltyped.
+    iApply ltyped_val_rec.
+    iApply ltyped_post_nil.
+    iApply ltyped_app.
+    { iApply (ltyped_lam []). iApply ltyped_post_nil. iApply ltyped_unit. }
+    iApply (ltyped_app _ _ _ _ _
+              (chan (<?? A> TY () ⊸ A; <!!> TY A; compute_type_service) ⊸ ())%lty).
+    {
+      simpl.
+      iApply (ltyped_lam [EnvItem "go" _]).
+      iApply ltyped_post_nil.
+      iApply ltyped_recv_texist; [ done | apply _ | ].
+      iIntros (Ys).
+      pose proof (ltys_S_inv Ys) as [A [Ys' HYs]].
+      pose proof (ltys_O_inv Ys') as HYs'.
+      rewrite HYs HYs' /=.
+      iApply ltyped_seq.
+      { iApply (ltyped_send _ [EnvItem "v" _; EnvItem "c" _; EnvItem "go" _]);
+          [ done | ].
+        iApply ltyped_app; [ by iApply ltyped_unit | ]=> /=.
+        by iApply ltyped_var. }
+      simpl.
+      iApply ltyped_app; [ by iApply ltyped_var | ].
+      simpl. rewrite !(Permutation_swap (EnvItem "go" _)).
+      iApply ltyped_subsumption; [ | | iApply env_le_refl | ].
+      { iApply env_le_cons; [ iApply lty_le_refl | iApply env_le_nil ]. }
+      { iApply lty_le_copy_elim. }
+      by iApply ltyped_var. }
+    iApply ltyped_app; [ by iApply ltyped_var | ].
+    iApply ltyped_subsumption; [ iApply env_le_nil | | iApply env_le_refl | ].
+    { iApply lty_le_arr; [ | iApply lty_le_refl ]. iApply lty_le_chan.
+      iApply lty_le_l; [ iApply lty_le_rec_unfold | iApply lty_le_refl ]. }
+    rewrite /compute_type_service_aux.
+    iApply ltyped_branch. intros x. rewrite -elem_of_dom. set_solver.
+  Qed.
+
+End compute_example.
